link: resolve admit, cleanup (works!)

link.v
@@ -72,7 +72,6 @@ Section Link_Template.
 
   Parameter findNext : val.
   Parameter decisiveOp : (dOp → val).
-  Parameter CCSSpec : (dOp → val).
   Parameter lockLoc : Node → loc.
   Parameter getLockLoc : val.
 
@@ -96,7 +95,7 @@ Section Link_Template.
       | SOME "n'" => unlockNode "n";; "tr" "n'" "k"
       end.
 
-  Definition CCSOp (Ψ: dOp) (root: Node) : val :=
+  Definition CSSOp (Ψ: dOp) (root: Node) : val :=
     rec: "dictOp" "k" :=
       let: "n" := traverse #root "k" in
       match: ((decisiveOp Ψ) "n" "k") with
@@ -105,7 +104,7 @@ Section Link_Template.
       end.
 
   (** Assumptions on the implementation made by the template proofs. *)
-  
+
   (* The node predicate is specific to each template implementation. See GRASShopper files
      b-link.spl and hashtbl-link.spl for the concrete definitions. *)
   Parameter node : Node → linkset_flowint_ur K → gset K → iProp.
@@ -124,13 +123,13 @@ Section Link_Template.
   (* The node-level invariant (γ in the paper).
    * See also link.spl for the matching GRASShopper definition *)
   Definition nodeinv I_n n: Prop :=
-    (∀ k, k ∈ linkset K I_n n ∧ ¬ in_outsets K k I_n → in_inset K k I_n n).    
+    (∀ k, k ∈ linkset K I_n n ∧ ¬ in_outsets K k I_n → in_inset K k I_n n).
 
-  (* The following hypothesis is proved as GRASShopper lemmas in 
+  (* The following hypothesis is proved as GRASShopper lemmas in
    * hashtbl-link.spl and b-link.spl *)
   Hypothesis node_implies_nodeinv : ∀ n I_n C,
-    (⌜✓I_n⌝)%I ∗ node n I_n C -∗ node n I_n C ∗ (⌜nodeinv I_n n⌝)%I. 
-   
+    (⌜✓I_n⌝)%I ∗ node n I_n C -∗ node n I_n C ∗ (⌜nodeinv I_n n⌝)%I.
+
   (** Coarse-grained specification *)
 
   Definition Ψ dop k (C: gset K) (C': gset K) (res: bool) : iProp :=
@@ -156,10 +155,10 @@ Section Link_Template.
 
   (* Todo: Can we simplify the match to ⌜b → in_inset k I_n n⌝? *)
   Parameter findNext_spec : ∀ (n: Node) (I_n : linkset_flowint_ur K) (C: gset K) (k: K),
-    ({{{ node n I_n C ∗ ⌜k ∈ linkset K I_n n ∨ in_inset K k I_n n⌝ }}}
+    ({{{ node n I_n C ∗ ⌜k ∈ inset K I_n n ∨ k ∈ linkset K I_n n⌝ }}}
       findNext #n #k
-    {{{ (b: bool) (n': Node), 
-        RET (match b with true => (SOMEV #n') | false => NONEV end); 
+    {{{ (b: bool) (n': Node),
+        RET (match b with true => (SOMEV #n') | false => NONEV end);
         node n I_n C ∗ (match b with true => ⌜in_outset K k I_n n'⌝ |
                                     false => ⌜¬in_outsets K k I_n⌝ end) }}})%I.
 
@@ -176,33 +175,36 @@ Section Link_Template.
 
   (** The concurrent search structure invariant *)
 
-  Definition CCS γ γ_fp γ_k γ_inr γ_fi root I C : iProp :=
-    (own γ (● I) ∗ own γ_k (● prod (KS, C)) ∗ own γ_fp (● domm I) ∗ ⌜globalinv K root I⌝
+  Definition CSS γ γ_fp γ_k γ_inr γ_fi root I C : iProp :=
+    (own γ (● I) ∗ own γ_k (● prod (KS, C)) ∗ own γ_fp (● domm I)
+    ∗ ⌜globalinv K root I⌝
     ∗ ([∗ set] n ∈ (domm I), (∃ (b: bool) (I_n: linkset_flowint_ur K),
       (lockLoc n) ↦ #b
       ∗ (if b then True
-        else (∃ C_n, node n I_n C_n ∗ own (γ_fi n) ((●{1/2} I_n)) ∗ own γ_k (◯ prod (keyset K I_n n, C_n))))
+        else (∃ C_n, node n I_n C_n ∗ own (γ_fi n) ((●{1/2} I_n))
+                     ∗ own γ_k (◯ prod (keyset K I_n n, C_n))))
       ∗ own γ (◯ I_n) ∗ ⌜domm I_n = {[n]}⌝ ∗ own (γ_fi n) ((●{1/2} I_n))
-      ∗ own (γ_inr n) (● (linkset K I_n n))))
-    )%I.    
+      ∗ own (γ_inr n) (● (inset K I_n n ∪ linkset K I_n n))))
+    )%I.
 
-  Definition is_CCS γ γ_fp γ_k γ_inr γ_fi root C :=
-    (∃ I, (CCS γ γ_fp γ_k γ_inr γ_fi root I C))%I.
+  Definition is_CSS γ γ_fp γ_k γ_inr γ_fi root C :=
+    (∃ I, (CSS γ γ_fp γ_k γ_inr γ_fi root I C))%I.
 
   (** Assorted useful lemmas *)
 
   Lemma globalinv_root_fp: ∀ I root, globalinv K root I → root ∈ domm I.
-  Proof. 
+  Proof.
     intros I root Hglob. unfold globalinv in Hglob.
     destruct Hglob as [H1 [H2 H3]]. done.
   Qed.
 
   Lemma globalinv_root_inr : ∀ I Ir root k,
-    globalinv K root I ∧ Ir ≼ I ∧ domm Ir = {[root]} → k ∈ linkset K Ir root.
+    globalinv K root I ∧ Ir ≼ I ∧ domm Ir = {[root]}
+    → k ∈ inset K Ir root ∨ k ∈ linkset K Ir root.
   Proof.
-    intros I Ir root k ((Hv & _ & _ & H6 & _) & [I2 Hincl] & Hdom).
+    intros I Ir root k ((Hv & _ & _ & Hl & _) & [I2 Hincl] & Hdom).
+    right. specialize (Hl k). destruct Hl.
     apply (linkset_monotone I Ir I2 k root); try done.
-    apply H6.
     set_solver.
   Qed.
 
@@ -250,7 +252,7 @@ Section Link_Template.
     iMod "AU" as (b) "[Hb HAU]". iDestruct "Hl" as %Hl.
     iEval (rewrite Hl) in "Hb". destruct b.
     - wp_cmpxchg_fail. iDestruct "HAU" as "[HAU _]".
-      iEval (rewrite Hl) in "HAU". 
+      iEval (rewrite Hl) in "HAU".
       iMod ("HAU" with "Hb") as "H".
       iModIntro. wp_pures. iApply "IH".
       iEval (rewrite <-Hl) in "H". done.
@@ -276,17 +278,18 @@ Section Link_Template.
     iModIntro. done.
   Qed.
 
-  
-  (** Proofs of traverse and CCSOp *)
+
+  (** Proofs of traverse and CSSOp *)
 
   Lemma traverse_spec (γ γ_fp γ_k: gname) (γ_inr γ_fi: Node → gname)
       (root: Node) (k: K) (n: Node) (Ns: gset Node) (I_n:linkset_flowint_ur K):
     ⌜n ∈ Ns⌝ ∗ own γ_fp (◯ Ns)
-    ∗ own (γ_inr n) (◯ (linkset K I_n n)) ∗ ⌜k ∈ linkset K I_n n⌝ -∗ 
-    <<< ∀ C, is_CCS γ γ_fp γ_k γ_inr γ_fi root C >>>
+    ∗ own (γ_inr n) (◯ (inset K I_n n ∪ linkset K I_n n))
+    ∗ ⌜k ∈ inset K I_n n ∨ k ∈ linkset K I_n n⌝ -∗
+    <<< ∀ C, is_CSS γ γ_fp γ_k γ_inr γ_fi root C >>>
       traverse #n #k @ ⊤
     <<< ∃ (n': Node) (Ns': gsetUR Node) (I_n': linkset_flowint_ur K) (Cn': gset K),
-        is_CCS γ γ_fp γ_k γ_inr γ_fi root C ∗ ⌜n' ∈ Ns'⌝
+        is_CSS γ γ_fp γ_k γ_inr γ_fi root C ∗ ⌜n' ∈ Ns'⌝
         ∗ own γ_fp (◯ Ns') ∗ node n' I_n' Cn' ∗ own (γ_fi n') ((●{1/2} I_n'))
         ∗ own γ_k (◯ prod (keyset K I_n' n', Cn')) ∗ ⌜domm I_n' = {[n']}⌝
         ∗ ⌜in_inset K k I_n' n'⌝ ∗ ⌜¬in_outsets K k I_n'⌝, RET #n' >>>.
@@ -307,15 +310,16 @@ Section Link_Template.
     iFrame "# % ∗". eauto with iFrame. } iIntros "(Hloc & ?)".
     destruct b. { iExFalso. done. } iModIntro.
     iPoseProof ((auth_set_incl (γ_inr n)) with "[$Hks $Hinrfp]") as "%".
-    iDestruct "Hkinr" as "%". assert (k ∈ linkset K In n) as Hkinr. { set_solver. }
+    iDestruct "Hkinr" as "%".
+    assert (k ∈ inset K In n ∨ k ∈ linkset K In n) as Hkinr; first by set_solver.
     iPoseProof (own_valid with "HIn") as "%". rename H2 into HInV.
     assert (✓ In) as HInv. { apply (auth_frag_valid (◯ In)). done. }
     iSplitR "Hb". iFrame "∗ % #". iExists I. iFrame "∗ % #". iApply "Hstar". iExists true, In.
     iFrame "# % ∗". iIntros "AU". iModIntro. wp_pures.
     iDestruct "Hb" as (Cn) "(Hrep & Hfil & Hks)". iDestruct "HNds" as %HNds.
     wp_bind (findNext _ _)%E. wp_apply ((findNext_spec n In Cn k) with "[Hrep]").
-    iFrame; iPureIntro; left; done. iIntros (b n') "(Hrep & Hb)". destruct b. 
-    - wp_pures. awp_apply (unlockNode_spec n). 
+    iFrame; iPureIntro; done. iIntros (b n') "(Hrep & Hb)". destruct b.
+    - wp_pures. awp_apply (unlockNode_spec n).
       iApply (aacc_aupd_abort with "AU"); first done. iIntros (C1) "Hst".
       iDestruct "Hst" as (I1) "(HI & HKS & HNDS & Hglob & Hstar)".
       iAssert (⌜n ∈ domm I1⌝)%I with "[HNDS]" as "%".
@@ -324,17 +328,17 @@ Section Link_Template.
       rewrite (big_sepS_delete _ (domm I1) n); last by eauto. iDestruct "Hstar" as "(Hcln & Hstar)".
       iDestruct "Hcln" as (b In1) "(Hlock & Hbb & HIn & #HNds1 & Hfis & Hks1)".
       destruct b; first last. { iDestruct "Hbb" as (Cn') "(Hrep' & _)".
-      iAssert (⌜False⌝)%I with "[Hrep Hrep']" as %Hf. { iApply (node_sep_star n In In1). 
+      iAssert (⌜False⌝)%I with "[Hrep Hrep']" as %Hf. { iApply (node_sep_star n In In1).
       iFrame. } exfalso. done. }
       iPoseProof ((own_valid_2 (γ_fi n) (●{1 / 2} In) (●{1 / 2} In1)) with "[Hfil] [Hfis]") as "%"; try done.
-      apply (auth_auth_frac_op_inv _ _ _ _) in H3. apply leibniz_equiv in H3. replace In1.            
+      apply (auth_auth_frac_op_inv _ _ _ _) in H3. apply leibniz_equiv in H3. replace In1.
       iDestruct "Hb" as %Hb. iDestruct "HNds1" as %HNds1. iDestruct "Hglob" as %Hglob.
       iPoseProof (auth_own_incl with "[$HI $HIn]") as (I2)"%".
       iPoseProof (own_valid with "HI") as "%". iAssert (⌜n' ∈ domm I1⌝)%I as "%".
       { iPureIntro. assert (n' ∈ domm I2).
         { apply (flowint_step I1 In I2 k n' root); try done. }
         assert (domm I1 = domm In ∪ domm I2).
-        { rewrite H4. apply flowint_comp_fp. 
+        { rewrite H4. apply flowint_comp_fp.
           rewrite H4 in H5 * => H5.
           rewrite <-H4.
           apply auth_auth_valid.
@@ -350,23 +354,25 @@ Section Link_Template.
           exists k. done. }
         rewrite HNds1 in H7. set_solver. }
       rewrite (big_sepS_delete _ (domm I1 ∖ {[n]}) n'); last first.
-      set_solver. iDestruct "Hstar" as "(Hcln' & Hstar)". 
+      set_solver. iDestruct "Hstar" as "(Hcln' & Hstar)".
       iDestruct "Hcln'" as (b In') "(Hlock' & Hbb' & HIn' & #HNds' & Hfis' & Hks1')".
       iPoseProof ((own_op γ (◯ In) (◯ In' )) with "[HIn HIn']") as "H"; first by eauto with iFrame.
       iPoseProof (own_valid with "H") as "%". rewrite -auth_frag_op in H7.
       assert (✓ (In ⋅ In')). { apply (auth_frag_valid (◯ (In ⋅ In'))). done. }
-      iDestruct "HNds'" as %HNds'. assert (k ∈ linkset K In' n').
+      iDestruct "HNds'" as %HNds'.
+      assert (k ∈ inset K In' n' ∨ k ∈ linkset K In' n').
       {
-        admit.
-        (* TODO need to adapt proof to new version of flowint_linkset_step.
-           I think one issue is that this proof assumes linkset is a superset
-           of inset, whereas the formulation in linkset_flows.v does not.
-           So maybe even the traverse spec might have to be updated. *)
-        (* apply (flowint_linkset_step (In⋅In') In In' k n n'); try done. *)
+        apply or_comm.
+        apply (flowint_linkset_step In In' k n'). done. set_solver.  
+        unfold in_outset in Hb. done.
       }
       assert (root ∈ domm I1). { apply globalinv_root_fp. done. } iDestruct "H" as "(HIn & HIn')".
-      iMod (own_update (γ_inr n') (● linkset K In' n') (● linkset K In' n' ⋅ ◯ linkset K In' n') with "Hks1'") as "HNs".
-      apply auth_update_core_id. apply gset_core_id. done. iDestruct "HNs" as "(Hks1' & #Hinr1')".
+      iMod (own_update (γ_inr n') _
+                       (● (inset K In' n' ∪ linkset K In' n')
+                          ⋅ ◯ (inset K In' n' ∪ linkset K In' n'))
+              with "Hks1'") as "HNs".
+      apply auth_update_core_id. 
+      apply gset_core_id. done. iDestruct "HNs" as "(Hks1' & #Hinr1')".
       iAaccIntro with "Hlock". { iIntros "Hlock". iModIntro. iSplitR "Hfil Hks Hrep". iFrame "∗ # %".
       iExists I1. iFrame "∗ % #". rewrite (big_sepS_delete _ (domm I1) n); last by eauto.
       iSplitR "Hstar Hbb' HIn' Hfis' Hks1' Hlock'". iExists true, In. iFrame "# % ∗".
@@ -382,16 +388,20 @@ Section Link_Template.
     - iApply fupd_wp. iMod "AU" as (C) "[Hst [_ Hclose]]". iSpecialize ("Hclose" $! n Ns In Cn).
       iMod ("Hclose" with "[Hst Hfil Hks Hrep Hb]") as "HΦ". iDestruct "Hb" as %Hnotout.
       iAssert (node n In Cn ∗ ⌜nodeinv In n⌝)%I with "[Hrep]" as "(Hrep & Hninv)".
-      { iApply (node_implies_nodeinv _ _ _). iFrame "∗ # %". } iDestruct "Hninv" as %Hninv.
-      iFrame "∗ # %". iPureIntro. unfold nodeinv in Hninv. specialize (Hninv k).
-      apply Hninv. try done. iModIntro. wp_pures. done.
-  Admitted.
+      { iApply (node_implies_nodeinv _ _ _). iFrame "∗ # %". }
+      iDestruct "Hninv" as %Hninv.
+      iFrame "∗ # %". iPureIntro. unfold nodeinv in Hninv.
+      destruct Hkinr.
+      * unfold in_inset. done.
+      * apply Hninv. split; try done.
+      * iModIntro. wp_pures. done.
+  Qed.
 
 
   (* Ghost state manipulation to make final proof cleaner *)
 
   (* Todo: I think k ∈ KS follows from k ∈ K1, so we can drop it here,
-    and in CCSOp_spec. *)
+    and in CSSOp_spec. *)
   Lemma ghost_update_keyset γ_k dop k Cn Cn' res K1 C:
     Ψ dop k Cn Cn' res ∗ own γ_k (● prod (KS, C)) ∗ own γ_k (◯ prod (K1, Cn))
     ∗ ⌜Cn' ⊆ K1⌝ ∗ ⌜k ∈ K1⌝ ∗ ⌜k ∈ KS⌝
@@ -402,16 +412,16 @@ Section Link_Template.
                 with "[$Ha $Hf]") as "%". iDestruct "HKS" as %HKS.
     iPoseProof ((own_valid γ_k (● prod (KS, C))) with "Ha") as "%".
     iPoseProof ((own_valid γ_k (◯ prod (K1, Cn))) with "Hf") as "%".
-    assert ((K1 = KS ∧ Cn = C) ∨ 
+    assert ((K1 = KS ∧ Cn = C) ∨
             (∃ a0 b0, KS = K1 ∪ a0 ∧ C = Cn ∪ b0 ∧ K1 ## a0 ∧ Cn ## b0 ∧ Cn ⊆ K1 ∧ C ⊆ KS ∧ b0 ⊆ a0)) as Hs.
     { apply (auth_ks_included K1 KS Cn C); try done. apply auth_auth_valid. done. }
     destruct Hs.
-    - iEval (unfold Ψ) in "HΨ". destruct H4. destruct dop. 
+    - iEval (unfold Ψ) in "HΨ". destruct H4. destruct dop.
       + iDestruct "HΨ" as "%". destruct H6.
         iModIntro. iExists C. iEval (rewrite <-H6) in "Hf". iFrame. unfold Ψ.
         iPureIntro. split; try done. rewrite <-H5. done.
       + iDestruct "HΨ" as "%". destruct H6. destruct res.
-        * iMod (own_update_2 γ_k (● prod (KS, C)) (◯ prod (K1, Cn)) 
+        * iMod (own_update_2 γ_k (● prod (KS, C)) (◯ prod (K1, Cn))
           (● prod (KS, C ∪ {[k]}) ⋅ ◯ prod (K1, Cn ∪ {[k]})) with "[Ha] [Hf]") as "(Ha & Hf)"; try done.
           { apply auth_update. apply auth_ks_local_update_insert.
             split; try done. apply auth_auth_valid. done.   }
@@ -420,7 +430,7 @@ Section Link_Template.
         * assert (Cn' = Cn). { set_solver. } iModIntro. iExists C. iEval (rewrite <-H8) in "Hf".
           iFrame. unfold Ψ. iPureIntro. rewrite <- H5. split; try done. rewrite H8 in H6. done.
       + iDestruct "HΨ" as "%". destruct H6. destruct res.
-        * iMod (own_update_2 γ_k (● prod (KS, C)) (◯ prod (K1, Cn)) 
+        * iMod (own_update_2 γ_k (● prod (KS, C)) (◯ prod (K1, Cn))
           (● prod (KS, C ∖ {[k]}) ⋅ ◯ prod (K1, Cn ∖ {[k]})) with "[Ha] [Hf]") as "(Ha & Hf)"; try done.
           { apply auth_update. apply auth_ks_local_update_delete. split; try done. apply auth_auth_valid. done. }
           iModIntro. iExists (C ∖ {[k]}). iEval (rewrite H6). iFrame.
@@ -432,7 +442,7 @@ Section Link_Template.
         iModIntro. iExists C. iEval (rewrite <-H11) in "Hf". iFrame. unfold Ψ.
         iPureIntro. split; try done. destruct res; set_solver.
       + iDestruct "HΨ" as "%". destruct H11. destruct res.
-        * iMod (own_update_2 γ_k (● prod (KS, C)) (◯ prod (K1, Cn)) 
+        * iMod (own_update_2 γ_k (● prod (KS, C)) (◯ prod (K1, Cn))
           (● prod (KS, C ∪ {[k]}) ⋅ ◯ prod (K1, Cn ∪ {[k]})) with "[Ha] [Hf]") as "(Ha & Hf)"; try done.
           { apply auth_update. apply auth_ks_local_update_insert. split; try done. }
           iModIntro. iExists (C ∪ {[k]}). iEval (rewrite H11). iFrame.
@@ -440,7 +450,7 @@ Section Link_Template.
         * assert (Cn' = Cn). { set_solver. } iModIntro. iExists C. iEval (rewrite <-H13) in "Hf".
           iFrame. unfold Ψ. iPureIntro. set_solver.
       + iDestruct "HΨ" as "%". destruct H11. destruct res.
-        * iMod (own_update_2 γ_k (● prod (KS, C)) (◯ prod (K1, Cn)) 
+        * iMod (own_update_2 γ_k (● prod (KS, C)) (◯ prod (K1, Cn))
           (● prod (KS, C ∖ {[k]}) ⋅ ◯ prod (K1, Cn ∖ {[k]})) with "[Ha] [Hf]") as "(Ha & Hf)"; try done.
           { apply auth_update. apply auth_ks_local_update_delete. split; try done. }
           iModIntro. iExists (C ∖ {[k]}). iEval (rewrite H11). iFrame.
@@ -449,30 +459,32 @@ Section Link_Template.
           iFrame. unfold Ψ. iPureIntro. set_solver.
   Qed.
 
-  (* ---------- Proofs of traverse and CCSOp ---------- *)
+  (** Verification of abstract specification of the search structure operation. *)
 
-  Theorem CCSOp_spec (γ γ_fp γ_k: gname) γ_inr γ_fi root (k: K) (dop: dOp):
-    ⌜k ∈ KS⌝ -∗ <<< ∀ C, is_CCS γ γ_fp γ_k γ_inr γ_fi root C >>>
-      CCSOp dop root #k @ ⊤
-    <<< ∃ C' (res: bool), is_CCS γ γ_fp γ_k γ_inr γ_fi root C' 
+  Theorem CSSOp_spec (γ γ_fp γ_k: gname) γ_inr γ_fi root (k: K) (dop: dOp):
+    ⌜k ∈ KS⌝ -∗ <<< ∀ C, is_CSS γ γ_fp γ_k γ_inr γ_fi root C >>>
+      CSSOp dop root #k @ ⊤
+    <<< ∃ C' (res: bool), is_CSS γ γ_fp γ_k γ_inr γ_fi root C'
         ∗ Ψ dop k C C' res, RET #res >>>.
   Proof.
     iIntros "HKin" (Φ) "AU". iLöb as "IH". wp_lam.
     iApply fupd_wp. iMod "AU" as (C0) "[Hst [HAU _]]".
     iDestruct "Hst" as (I0) "(HI & HKS & HNDS & #Hglob & Hstar)".
-    iDestruct "Hglob" as %Hglob. iDestruct "HKin" as %HKin. 
+    iDestruct "Hglob" as %Hglob. iDestruct "HKin" as %HKin.
     assert (root ∈ domm I0)%I as Hroot. { apply globalinv_root_fp. done. }
     iMod (own_update γ_fp (● domm I0) (● domm I0 ⋅ ◯ domm I0) with "HNDS") as "H".
-    { apply auth_update_core_id. apply gset_core_id. done. } 
+    { apply auth_update_core_id. apply gset_core_id. done. }
     iDestruct "H" as "(HNDS & #Hfp0)".
     rewrite (big_sepS_elem_of_acc _ (domm I0) root); last by eauto.
     iDestruct "Hstar" as "[Hn Hstar]".
     iDestruct "Hn" as (b Ir) "(H1 & H2 & H3 & H4 & H5 & Hksr)".
     iPoseProof (auth_own_incl with "[$HI $H3]") as "%". iDestruct "H4" as %HNdsr.
-    (*assert (inreach Ir root = inreach I0 root) as Hinreach. { apply globalinv_inreach; try done. }*)
-    iMod (own_update (γ_inr root) (● linkset K Ir root) (● linkset K Ir root ⋅ ◯ linkset K Ir root) with "Hksr") as "H".
+    iMod (own_update (γ_inr root) _
+                     (● (inset K Ir root ∪ linkset K Ir root)
+                      ⋅ ◯ (inset K Ir root ∪ linkset K Ir root))
+            with "Hksr") as "H".
     apply auth_update_core_id. apply gset_core_id. done. iDestruct "H" as "(Hksr & #Hinr)".
-    iMod ("HAU" with "[HI HKS H1 H2 H3 H5 Hstar HNDS Hksr] ") as "AU". 
+    iMod ("HAU" with "[HI HKS H1 H2 H3 H5 Hstar HNDS Hksr] ") as "AU".
     { iExists I0. iFrame "∗ % #". iApply "Hstar". iExists b, Ir. iFrame "∗ # %". }
     iModIntro. wp_bind (traverse _ _)%E.
     awp_apply (traverse_spec γ γ_fp γ_k γ_inr γ_fi root k root (domm I0) Ir). iFrame "∗ # %".
@@ -488,7 +500,7 @@ Section Link_Template.
       wp_pures. wp_bind(unlockNode _)%E.
       awp_apply (unlockNode_spec n).
       iApply (aacc_aupd_commit with "AU"); first done. iIntros (C2) "Hst".
-      iDestruct "Hst" as (I) "(HI & HKS & HNDS & #Hglob & Hstar)". 
+      iDestruct "Hst" as (I) "(HI & HKS & HNDS & #Hglob & Hstar)".
       iDestruct "Hglob" as %Hglob'.
       iAssert (⌜n ∈ domm I⌝)%I with "[HNDS]" as "%".
       { iPoseProof ((auth_set_incl γ_fp Ns (domm I)) with "[$]") as "%".
@@ -497,10 +509,10 @@ Section Link_Template.
       iDestruct "Hstar" as "[Hn Hstar]".
       iDestruct "Hn" as (b' In1) "(Hlock & Hb & HIn & #HNds & Hfis & Hinreach)".
       destruct b'; first last. { iDestruct "Hb" as (Cn'') "(Hrep' & _)".
-      iAssert (⌜False⌝)%I with "[Hrep Hrep']" as %Hf. { iApply (node_sep_star n In In1). 
+      iAssert (⌜False⌝)%I with "[Hrep Hrep']" as %Hf. { iApply (node_sep_star n In In1).
       iFrame. } exfalso. done. }
       iAaccIntro with "Hlock". { iIntros "Hlock". iModIntro. iSplitR "Hfil Hrep Hks".
-      iExists I. iFrame "∗ % #". iApply "Hstar". iExists true, In1. 
+      iExists I. iFrame "∗ % #". iApply "Hstar". iExists true, In1.
       iFrame "∗ # %". eauto with iFrame. } iIntros "Hlock".
       iPoseProof (auth_own_incl with "[$HI $HIn]") as (I2)"%".
       iPoseProof ((own_valid γ (● I)) with "HI") as "%".
@@ -508,19 +520,19 @@ Section Link_Template.
       apply (auth_auth_frac_op_inv _ _ _ _) in H3. apply leibniz_equiv in H3. replace In1.
       iPoseProof ((own_valid γ (◯ In)) with "HIn") as "%". rename H4 into HInV.
       assert (✓ In) as HInv. { apply (auth_frag_valid (◯ In)). done. }
-      iAssert (node n In Cn' ∗ ⌜nodeinv In n⌝)%I with "[Hrep]" as "(Hrep & Hninv)". 
-      { iApply (node_implies_nodeinv _ _ _). iFrame "% ∗ #". } iDestruct "Hninv" as %Hninv.                   
+      iAssert (node n In Cn' ∗ ⌜nodeinv In n⌝)%I with "[Hrep]" as "(Hrep & Hninv)".
+      { iApply (node_implies_nodeinv _ _ _). iFrame "% ∗ #". } iDestruct "Hninv" as %Hninv.
       iMod ((ghost_update_keyset γ_k dop k Cn Cn' res (keyset K In n) C2) with "[HKS Hks]") as "Hgks".
       iFrame "% ∗ #". iPureIntro. apply keyset_def; try done.
       iDestruct "Hgks" as (C2') "(#HΨC & Ha & Hf)".
       iModIntro. iExists (C2'), res. iSplitL. iSplitR "HΨC".
       { iExists I. iFrame "∗ % #".
-      iApply "Hstar". iExists false, In. 
+      iApply "Hstar". iExists false, In.
       iFrame "∗ % #". iExists Cn'. eauto with iFrame. } done.
       iIntros "HΦ". iModIntro. wp_pures. done.
     - wp_match. awp_apply (unlockNode_spec n).
       iApply (aacc_aupd_abort with "AU"); first done. iIntros (C2) "Hst".
-      iDestruct "Hst" as (I) "(HI & HKS & HNDS & #Hglob & Hstar)". 
+      iDestruct "Hst" as (I) "(HI & HKS & HNDS & #Hglob & Hstar)".
       iDestruct "Hglob" as %Hglob'.
       iAssert (⌜n ∈ domm I⌝)%I with "[HNDS]" as "%".
       { iPoseProof ((auth_set_incl γ_fp Ns (domm I)) with "[$]") as "%".
@@ -529,15 +541,15 @@ Section Link_Template.
       iDestruct "Hstar" as "[Hn Hstar]".
       iDestruct "Hn" as (b' In1) "(Hlock & Hb' & HIn & #HNds & Hfis & Hinreach)".
       destruct b'; first last. { iDestruct "Hb'" as (Cn'') "(Hrep' & _)".
-      iAssert (⌜False⌝)%I with "[Hb Hrep']" as %Hf. { iApply (node_sep_star n In In1). 
+      iAssert (⌜False⌝)%I with "[Hb Hrep']" as %Hf. { iApply (node_sep_star n In In1).
       iFrame "∗ # %". } exfalso. done. }
       iAaccIntro with "Hlock". { iIntros "Hlock". iModIntro. iSplitR "Hfil Hb Hks".
-      iExists I. iFrame "∗ % #". iApply "Hstar". iExists true, In1. 
+      iExists I. iFrame "∗ % #". iApply "Hstar". iExists true, In1.
       iFrame "∗ # %". eauto with iFrame. } iIntros "Hlock". iModIntro.
       iPoseProof ((own_valid_2 (γ_fi n) (●{1 / 2} In) (●{1 / 2} In1)) with "[Hfil] [Hfis]") as "%"; try done.
-      apply (auth_auth_frac_op_inv _ _ _ _) in H1. apply leibniz_equiv in H1. replace In1.            
+      apply (auth_auth_frac_op_inv _ _ _ _) in H1. apply leibniz_equiv in H1. replace In1.
       iSplitR "". iExists I. iFrame "∗ % #". iApply "Hstar". iExists false, In. iFrame "∗ % #".
       iExists Cn. iFrame. iIntros "AU". iModIntro. wp_pures. iApply "IH"; try done.
   Qed.
- 
+
 End Link_Template.
